Update IO/QExp with the new things from STLC/QExp

rupicola/io/QExp.fst
@@ -15,18 +15,12 @@ val helper_var0 :
 let helper_var0 g a fsG = hd fsG
 
 unfold
-val helper_var1 : g:typ_env ->
+val helper_varS : g:typ_env ->
                   a:qType ->
                   b:qType ->
-                  fs_oexp (extend b (extend a g)) a
-let helper_var1 g a b fsG = hd (tail fsG)
-unfold
-val helper_var2 : g:typ_env ->
-                  a:qType ->
-                  b:qType ->
-                  c:qType ->
-                  fs_oexp (extend c (extend b (extend a g))) a
-let helper_var2 g a b c fsG = hd (tail (tail fsG))
+                  fs_oexp g a ->
+                  fs_oexp (extend b g) a
+let helper_varS g a b x fsG = x (tail fsG)
 
 unfold
 val helper_unit : g:typ_env -> fs_oexp g qUnit
@@ -132,15 +126,13 @@ type exp_quotation : #a:qType -> g:typ_env -> fs_oexp g a -> Type =
                 #a : qType ->
                 exp_quotation _ (helper_var0 g a)
 
-| QVar1       : #g : typ_env ->
+| QVarS       : #g : typ_env ->
                 #a : qType ->
                 #b : qType ->
-                exp_quotation _ (helper_var1 g a b)
-| QVar2       : #g : typ_env ->
-                #a : qType ->
-                #b : qType ->
-                #c : qType ->
-                exp_quotation _ (helper_var2 g a b c)
+                #x : fs_oexp g a ->
+                exp_quotation g x ->
+                exp_quotation _ (helper_varS g a b x)
+
 (** we need a case for each deBrujin variable **)
 
 | QApp        : #g : typ_env ->
@@ -285,11 +277,11 @@ let test_var0
 
 let test_var1
   : exp_quotation #qBool (extend qBool (extend qBool empty)) var1
-  = QVar1
+  = QVarS QVar0
 
 let test_var2
   : exp_quotation #qBool (extend qBool (extend qBool (extend qBool empty))) var2
-  = QVar2
+  = QVarS (QVarS QVar0)
 
 let test_constant
   : closed_exp_quotation (qBool ^-> qBool) constant
@@ -305,11 +297,11 @@ let test_thunked_id
 
 let test_proj1
   : closed_exp_quotation (qBool ^-> qBool ^-> qBool ^-> qBool) proj1
-  = QLambda (QLambda (QLambda QVar2))
+  = QLambda (QLambda (QLambda (QVarS (QVarS QVar0))))
 
 let test_proj2
   : closed_exp_quotation (qBool ^-> qBool ^-> qBool ^-> qBool) proj2
-  = QLambda (QLambda (QLambda QVar1))
+  = QLambda (QLambda (QLambda (QVarS QVar0)))
 
 let test_proj3
   : closed_exp_quotation (qBool ^-> qBool ^-> qBool ^-> qBool) proj3
@@ -328,7 +320,7 @@ let test_apply_top_level_def'
   = QLambda (QLambda (QApp
                       (QApp #_ #_ #_ #(fun _ x y -> y)
                         (QLambda (QLambda QVar0))
-                        QVar1)
+                        (QVarS QVar0))
                       QVar0))
 
 let test_papply__top_level_def
@@ -361,11 +353,11 @@ let test_negb
 
 let test_negb_pred
   : closed_exp_quotation ((qBool ^-> qBool) ^-> qBool ^-> qBool) negb_pred
-  = QLambda (QLambda (QIf (QApp QVar1 QVar0) QFalse QTrue))
+  = QLambda (QLambda (QIf (QApp (QVarS QVar0) QVar0) QFalse QTrue))
 
 let test_if2
   : closed_exp_quotation (qBool ^-> qBool ^-> qBool) if2
-  = QLambda (QLambda (QIf QVar1 QFalse QVar0))
+  = QLambda (QLambda (QIf (QVarS QVar0) QFalse QVar0))
 
 (** Because of the fancy types, now one needs a preprocessing tactic to
     get rid of the qTypes **)
@@ -378,19 +370,19 @@ let simplify_qType (x:term) : Tac term =
 let test_callback_return
   : closed_exp_quotation (qBool ^-> (qBool ^-> qBool)) callback_return
   = QLambda (QIf QVar0
-                       (QLambda #_ #_ #_ #(fun fsG y -> hd fsG) QVar1) // TODO: why cannot it infer myf?
+                       (QLambda #_ #_ #_ #(fun fsG y -> hd fsG) (QVarS QVar0)) // TODO: why cannot it infer myf?
                        (QLambda #_ #_ #_ #(fun fsG z -> z) QVar0))
 
 [@@ (preprocess_with simplify_qType)]
 let test_callback_return'
   : closed_exp_quotation (qBool ^-> (qBool ^-> qBool)) callback_return'
   = QLambda (QIf QVar0
-                       (QLambda #_ #_ #_ #(fun fsG y -> hd fsG) QVar1)
+                       (QLambda #_ #_ #_ #(fun fsG y -> hd fsG) (QVarS QVar0))
                        (QLambda #_ #_ #_ #(fun fsG -> identity) QVar0)) // TODO: why does it not work to unfold identity here?
 
 let test_make_pair
   : closed_exp_quotation (qBool ^-> qBool ^-> (qBool ^* qBool)) make_pair
-  = QLambda (QLambda (QMkpair QVar1 QVar0))
+  = QLambda (QLambda (QMkpair (QVarS QVar0) QVar0))
 
 // TODO: why does this fail?
 [@@ (preprocess_with simplify_qType)]
@@ -400,7 +392,6 @@ let test_pair_of_functions ()
   by (norm [delta_only [`%pair_of_functions]];
       norm [delta_only [`%fs_oexp; `%qUnit; `%qBool; `%op_Hat_Subtraction_Greater; `%op_Hat_Star; `%op_Hat_Subtraction_Greater_Bang_At; `%get_rel; `%get_Type; `%Mkdtuple2?._1;`%Mkdtuple2?._2];iota];
      // trefl (); //this fails
-     dump "H";
      tadmit ())
   =  QMkpair
       (QLambda (QApp #_ #_ #_ #(fun _ x -> if x then false else true)
@@ -414,7 +405,7 @@ let test_pair_of_functions2
     pair_of_functions2
   = admit (); QMkpair // TODO
       (QLambda (QIf QVar0 QFalse QTrue))
-      (QLambda (QLambda (QIf QVar1 QFalse QVar0)))
+      (QLambda (QLambda (QIf (QVarS QVar0) QFalse QVar0)))
 
 let test_fst_pair
   : closed_exp_quotation (qBool) fst_pair
@@ -479,12 +470,13 @@ let test_apply_io_bind_identity
 let test_apply_io_bind_pure_if ()
   : Tot (closed_exp_quotation (qBool ^->!@ qBool) apply_io_bind_pure_if)
     by (
-      set_guard_policy Goal;
+      // TODO: why?
       norm [delta_only [`%apply_io_bind_pure_if]];
-      split (); trefl (); explode (); trefl ();
-      explode ();
       norm [delta_only [`%op_Hat_Subtraction_Greater_Bang_At]];
-      trefl ())
+      set_guard_policy Goal;
+      split (); trefl ();
+      explode (); trefl ();
+      explode (); trefl ())
   = QLambdaIO
       (QBind
         (QReturn QVar0)
@@ -516,7 +508,7 @@ let test_apply_io_bind_read_if_write
   : closed_io_exp_quotation _ apply_io_bind_read_if_write
   = QBind
       (QAppIO QRead Qtt)
-      (QLambdaIO (** TODO: weird that this does not require the lambda as the other examples **)
+      (QLambdaIO
         (QIfIO QVar0
           (QAppIO QWrite QFalse)
           (QAppIO QWrite QTrue)))
